Starting updating SMC proof to take account of EasyCrypt match statement and other changes, some of which are planned.

smc-next/Forward.ec
@@ -25,7 +25,7 @@ axiom fwd_pi_uniq : uniq [adv_pi; 0].
    asking to forward u to pt2 *)
 
 op fw_req (func : addr, pt1 pt2 : port, u : univ) : msg =
-     (Dir, (func, 1), pt1, UnivPair (UnivPort pt2, u)).
+     (Dir, (func, 1), pt1, UnivPair (UnivPort pt2) u).
 
 op dec_fw_req (m : msg) : (addr * port * port * univ) option =
      let (mod, pt1, pt2, v) = m
@@ -38,7 +38,11 @@ op dec_fw_req (m : msg) : (addr * port * port * univ) option =
 
 lemma enc_dec_fw_req (func : addr, pt1 pt2 : port, u : univ) :
   dec_fw_req (fw_req func pt1 pt2 u) = Some (func, pt1, pt2, u).
-proof. done. qed.
+proof.
+by rewrite /dec_fw_req /fw_req /= (is_univ_pair (UnivPort pt2) u)
+           /= enc_dec_univ_pair oget_some /= (is_univ_port pt2) /=
+           enc_dec_univ_port.
+qed.
 
 lemma dec_enc_fw_req (m : msg, func : addr, pt1 pt2 : port, u : univ) :
   dec_fw_req m = Some (func, pt1, pt2, u) =>
@@ -52,12 +56,12 @@ move => [#] -> pt1'_2 iup_u'.
 have [] p : exists (p : univ * univ), dec_univ_pair u' = Some p.
   exists (oget (dec_univ_pair u')); by rewrite -some_oget.
 case p => v1 v2 /dec_enc_univ_pair -> /=.
-rewrite oget_some /=.
+rewrite enc_dec_univ_pair oget_some /=.
 case (is_univ_port v1) => // iupt_v1.
 have [] pt3 : exists pt3, dec_univ_port v1 = Some pt3.
   exists (oget (dec_univ_port v1)); by rewrite -some_oget.
 move => /dec_enc_univ_port => -> /=.
-rewrite oget_some /#.
+rewrite enc_dec_univ_port oget_some /#.
 qed.
 
 op is_fw_req (m : msg) : bool =
@@ -65,7 +69,9 @@ op is_fw_req (m : msg) : bool =
 
 lemma is_fw_req (func : addr, pt1 pt2 : port, u : univ) :
   is_fw_req (fw_req func pt1 pt2 u).
-proof. done. qed.
+proof.
+by rewrite /is_fw_req enc_dec_fw_req.
+qed.
 
 lemma dest_good_fw_req (m : msg) :
   is_fw_req m =>
@@ -92,7 +98,7 @@ qed.
    completing the forwarding of u that was requested by pt1 *)
 
 op fw_rsp (func : addr, pt1 pt2 : port, u : univ) : msg =
-     (Dir, pt2, (func, 1), UnivPair (UnivPort pt1, u)).
+     (Dir, pt2, (func, 1), UnivPair (UnivPort pt1) u).
 
 op dec_fw_rsp (m : msg) : (addr * port * port * univ) option =
      let (mod, pt1, pt2, v) = m
@@ -105,7 +111,11 @@ op dec_fw_rsp (m : msg) : (addr * port * port * univ) option =
 
 lemma enc_dec_fw_rsp (func : addr, pt1 pt2 : port, u : univ) :
   dec_fw_rsp (fw_rsp func pt1 pt2 u) = Some (func, pt1, pt2, u).
-proof. done. qed.
+proof.
+by rewrite /dec_fw_rsp /fw_rsp /= (is_univ_pair (UnivPort pt1) u) /=
+           (enc_dec_univ_pair (UnivPort pt1) u) /= oget_some /=
+           (is_univ_port pt1) /= enc_dec_univ_port.
+qed.
 
 lemma dec_enc_fw_rsp (m : msg, func : addr, pt1 pt2 : port, u : univ) :
   dec_fw_rsp m = Some (func, pt1, pt2, u) =>
@@ -119,12 +129,12 @@ move => [#] -> pt2'_2 iup_u'.
 have [] p : exists (p : univ * univ), dec_univ_pair u' = Some p.
   exists (oget (dec_univ_pair u')); by rewrite -some_oget.
 case p => v1 v2 /dec_enc_univ_pair -> /=.
-rewrite oget_some /=.
+rewrite enc_dec_univ_pair oget_some /=.
 case (is_univ_port v1) => // iupt_v1.
 have [] pt3 : exists pt3, dec_univ_port v1 = Some pt3.
   exists (oget (dec_univ_port v1)); by rewrite -some_oget.
 move => /dec_enc_univ_port => -> /=.
-rewrite oget_some /#.
+rewrite enc_dec_univ_port oget_some /#.
 qed.
 
 op is_fw_rsp (m : msg) : bool =
@@ -132,7 +142,9 @@ op is_fw_rsp (m : msg) : bool =
 
 lemma is_fw_rsp (func : addr, pt1 pt2 : port, u : univ) :
   is_fw_rsp (fw_rsp func pt1 pt2 u).
-proof. done. qed.
+proof.
+by rewrite /is_fw_rsp enc_dec_fw_rsp.
+qed.
 
 lemma dest_good_fw_rsp (m : msg) :
   is_fw_rsp m => (oget (dec_fw_rsp m)).`3 = m.`2.
@@ -170,8 +182,9 @@ lemma enc_dec_fw_obs (func adv : addr, pt1 pt2 : port, u : univ) :
   dec_fw_obs (fw_obs func adv pt1 pt2 u) = Some (func, adv, pt1, pt2, u).
 proof.
 by rewrite /fw_obs /dec_fw_obs /=
-   (is_univ_triple (UnivPort pt2) (UnivPort pt2) u) /=
-    enc_dec_univ_triple.
+           (is_univ_triple (UnivPort pt2) (UnivPort pt2) u) /=
+           enc_dec_univ_triple oget_some /= (is_univ_port pt1) /=
+           !enc_dec_univ_port.
 qed.
 
 lemma dec_enc_fw_obs (m : msg, func adv : addr, pt1 pt2 : port, u : univ) :
@@ -257,41 +270,9 @@ qed.
 
 type fw_state = [
     FwStateInit
-  | FwStateWait  of (port * port * univ)
-  | FwStateFinal of (port * port * univ)
+  | FwStateWait  of port & port & univ
+  | FwStateFinal of port & port & univ
 ].
-
-op dec_fw_state_wait (st : fw_state) : (port * port * univ) option =
-     with st = FwStateInit    => None
-     with st = FwStateWait t  => Some t
-     with st = FwStateFinal _ => None.
-
-lemma enc_dec_fw_state_wait (t : port * port * univ) :
-  dec_fw_state_wait (FwStateWait t) = Some t.
-proof. done. qed.
-
-op is_fw_state_wait (st : fw_state) : bool =
-  dec_fw_state_wait st <> None.
-
-lemma is_fw_state_wait (t : port * port * univ) :
-  is_fw_state_wait (FwStateWait t).
-proof. done. qed.
-
-op dec_fw_state_final (st : fw_state) : (port * port * univ) option =
-     with st = FwStateInit    => None
-     with st = FwStateWait _  => None
-     with st = FwStateFinal x => Some x.
-
-lemma enc_dec_fw_final (t : port * port * univ) :
-  dec_fw_state_final (FwStateFinal t) = Some t.
-proof. done. qed.
-
-op is_fw_state_final (st : fw_state) : bool =
-  dec_fw_state_final st <> None.
-
-lemma is_fw_state_final (t : port * port * univ) :
-  is_fw_state_final (FwStateFinal t).
-proof. done. qed.
 
 module Forw : FUNC = {
   var self, adv : addr
@@ -305,27 +286,35 @@ module Forw : FUNC = {
     var pt1, pt2 : port; var u : univ;
     var addr1, addr2 : addr;
     var r : msg option <- None;
-    if (st = FwStateInit) {
-      if (is_fw_req m) {
-        (addr1, pt1, pt2, u) <- oget (dec_fw_req m);
-        if (self = addr1 /\
-            ! self <= pt1.`1 /\ ! self <= pt2.`1 /\
-            ! adv <= pt1.`1 /\ ! adv <= pt2.`1) {
-          r <- Some (fw_obs self adv pt1 pt2 u);
-          st <- FwStateWait (pt1, pt2, u);
-        }
+    match st with
+      FwStateInit => {
+        match dec_fw_req m with
+          Some x => {
+            (addr1, pt1, pt2, u) <- x;
+            if (self = addr1 /\
+                ! self <= pt1.`1 /\ ! self <= pt2.`1 /\
+                ! adv <= pt1.`1 /\ ! adv <= pt2.`1) {
+              r <- Some (fw_obs self adv pt1 pt2 u);
+              st <- FwStateWait pt1 pt2 u;
+            }
+          }
+        | None => { }
+        end;
       }
-    }
-    elif (is_fw_state_wait st) {
-      (pt1, pt2, u) <- oget (dec_fw_state_wait st);
-      if (is_fw_ok m) {
-        (addr1, addr2) <- oget (dec_fw_ok m);
-        if (addr1 = self) {
-          r <- Some (fw_rsp self pt1 pt2 u);
-          st <- FwStateFinal (pt1, pt2, u);
-        }
+    | FwStateWait pt1 pt2 u => {
+        match dec_fw_ok m with
+          Some x => {
+            (addr1, addr2) <- x;
+            if (addr1 = self) {
+              r <- Some (fw_rsp self pt1 pt2 u);
+              st <- FwStateFinal pt1 pt2 u;
+            }
+          }
+        | None => { }
+        end;
       }
-    }
+    | FwStateFinal _ _ _ => { }
+    end;
     return r;
   }
 }.
@@ -334,17 +323,24 @@ module Forw : FUNC = {
 
 op term_metric_max : int = 2.
 
-op term_metric (st : fw_state) : int =
-     with st = FwStateInit    => 2
-     with st = FwStateWait _  => 1
-     with st = FwStateFinal _ => 0.
+(* FIXME when better glob type
 
-lemma ge0_term_metric (st : fw_state) : 0 <= term_metric st.
-proof. by case st. qed.
+   print glob Forw:
+   1: Forw.st : fw_state
+   2: Forw.adv : addr
+   3: Forw.self : addr *)
 
-lemma term_metric_is_fw_state_wait (st : fw_state) :
-  is_fw_state_wait st => term_metric st = 1.
-proof. by case st. qed.
+op term_metric (g : glob Forw) : int =
+     match g.`1 with
+       FwStateInit        => 2
+     | FwStateWait _ _ _  => 1
+     | FwStateFinal _ _ _ => 0
+     end.
+
+lemma ge0_term_metric (g : glob Forw) : 0 <= term_metric g.
+proof.
+smt().
+qed.
 
 lemma init :
   equiv
@@ -359,7 +355,7 @@ lemma term_init :
   [Forw.init ~ Forw.init :
    ={self_, adv_} ==>
    ={res, glob Forw} /\
-   term_metric Forw.st{1} = term_metric_max].
+   term_metric (glob Forw){1} = term_metric_max].
 proof.
 proc; auto.
 qed.
@@ -368,26 +364,25 @@ lemma term_invoke (n : int) :
   equiv
   [Forw.invoke ~ Forw.invoke :
    ={m, glob Forw} /\
-   term_metric Forw.st{1} = n ==>
-   ={res, Forw.st} /\
-   (res{1} = None \/ term_metric Forw.st{1} = n - 1)].
+   term_metric (glob Forw){1} = n ==>
+   ={res, glob Forw} /\
+   (res{1} = None \/ term_metric (glob Forw){1} < n)].
 proof.
 proc; sp 1 1.
-if => //.
-if => //.
+match => //.
+match => // x y.
 sp 1 1.
-if; first by move => |> &1 &2 <-.
-auto => |> &1 &2 <- //.
+if; first move => |> &1 &2 -> //.
+auto => |> &1 &2 -> //.
 auto.
-if => //.
-sp 1 1.
-if => //.
+move => pt1 pt2 u pt1' pt2' u'.
+match => // x y.
 sp 1 1.
 if.
-move => &1 &2 [#] oget_dec_1 oget_dec_2 _ _ _ _ ->>.
-rewrite -oget_dec_1 /= in oget_dec_2.
-by elim oget_dec_2 => -> _.
-auto => |> &1 &2.
-smt(term_metric_is_fw_state_wait).
+(*FIXME - use better crush*)
+move => &1 &2 [#] *.
+move : H7 H1 H2 H H0 H10.
+move => -> -> /= -> <- [#] -> _ -> //.
+auto.
 auto.
 qed.
